ml_sources/examples/snapshot_isolation/examples/deprecated/anomalie/anomalie_runner.ml
@@ -1,4 +1,4 @@
-open Unix
+(* open Unix
 open Ast
 open !Anomalie_code
 
@@ -30,4 +30,4 @@ let runner () =
   then node_check_account (clt_addr 4) (clt_addr 5) srv_addr
   else assert false
 
-let () = runner ()
+let () = runner () *)
