aneris/examples/snapshot_isolation/examples/sequential_writes/sequential_writes_proof.v
@@ -12,7 +12,7 @@ From aneris.aneris_lang.program_logic Require Import
      aneris_weakestpre aneris_adequacy aneris_lifting.
 From iris.base_logic.lib Require Import invariants.
 From aneris.examples.snapshot_isolation.examples.sequential_writes 
-  Require Import sequential_writes_code.
+  Require Import sequential_writes_code_exp.
 Import ser_inj.
 From aneris.examples.snapshot_isolation.instantiation
      Require Import snapshot_isolation_api_implementation.
@@ -130,97 +130,67 @@ Context `{!anerisG Mdl Σ, !SI_resources Mdl Σ, !SI_client_toolbox, !KVSG Σ}.
     rewrite /transaction2_client. wp_pures. rewrite Hip Hports.
     wp_apply (SI_init_client_proxy_spec with "[$Hunalloc $Hprot $Hmsghis $Hports]").
     iIntros (rpc) "Hcstate". wp_pures. rewrite /transaction2. wp_pures.
-    wp_apply (SI_start_spec $! rpc client_2_addr (⊤ ∖ ↑client_inv_name)); try solve_ndisj.
-    iInv (client_inv_name) as ">[%hx [Hkx [(_ & _ & Htok') | Hrest]]]" "HClose";
-    try iDestruct (token_exclusive with "Htok Htok'") as "[]".
-    iModIntro. iFrame.
-    iExists {["x" := hx]}.
-    rewrite !big_sepM_insert; try set_solver.
-    rewrite big_sepM_empty.
-    iSplitL "Hkx"; first iFrame.
-    iNext. iIntros "(Hcstate & [Hkx _] & [Hcx _] & Hseen & _)".
-    iMod ("HClose" with "[Hkx Hrest]") as "_".
-    { iNext. iExists hx. iFrame. }
-    iModIntro. wp_pures.
-    wp_apply (simplified_wait_on_keyT_spec _ _ (#1) _ 
-      {["x":= hx]} _ (⊤ ∖ ↑client_inv_name) 
-      (λ m, ⌜m = {["x":=[(#1)]]}⌝ ∗ token γF2)%I (token γF2) (token γF1)
-      with "[] [] [] [] [] [] [Hcx Hcstate Hseen Htok] [HΦ]");
-    try solve_ndisj; try iPureIntro; try set_solver.
-      - iModIntro. iIntros (h) "(Hxseen & Htok)". 
-        iInv (client_inv_name) as ">[%hx' [Hkx [(_ & _ & Htok') | [(-> & Htok') | ->]]]]" "HClose".
-        + iDestruct (token_exclusive with "Htok Htok'") as "[]".
-        + iModIntro. iExists {["x":= [(#1)]]}.
-          iSplit. 
-          { iPureIntro. set_solver. }
-          iSplitL "Hkx".
-          { rewrite !big_sepM_insert; set_solver. }
-          iSplitL "Htok".
-          { by iFrame. }
-          iFrame. iIntros "!> [Hkx Htok]". 
-          iMod ("HClose" with "[Htok Hkx]") as "_"; try done.
-          iNext. iExists _. 
-          rewrite !(big_sepM_insert); try set_solver.
-          iDestruct "Hkx" as "[Hkx _]". iFrame.
-          iRight. iLeft. by iFrame.
-          + iDestruct (Seen_valid (⊤ ∖ ↑client_inv_name) with "[]") as "Hfalse"; 
-          [solve_ndisj|iApply SI_GlobalInv|].
-          iMod ("Hfalse" with "[$Hxseen $Hkx]") as "(Hkx & %Hfalse)".
-          destruct Hfalse as [? Hfalse].
-          by apply app_cons_not_nil in Hfalse.
-      - iModIntro. 
-        iInv (client_inv_name) as ">[%hx' [Hkx Hrest]]" "HClose".
-        iModIntro.
-        iExists {["x":= hx']}.
-        iSplit. 
-        { iPureIntro. set_solver. }
-        iSplitL "Hkx".
-        { rewrite !big_sepM_insert; set_solver. }
-        iIntros "!> Hkx". 
-        iMod ("HClose" with "[Hkx Hrest]") as "_"; try done.
-        iNext. iExists _. 
-        rewrite !(big_sepM_insert); try set_solver.
-        iDestruct "Hkx" as "[Hkx _]". iFrame.
-      - iIntros (v Φ') "!>Htrue HΦ".
-        wp_lam. wp_op.
-        apply bin_op_eval_eq_val.
-        case_bool_decide as Heq;
-        iApply "HΦ"; set_solver.
-      - rewrite !(big_sepM_insert); try set_solver.
-        rewrite !big_sepM_empty. iFrame.
-      - iNext. iIntros (ms) "(%Hdom & (-> & Htok) & Hcp & Hx & Hseen)".
-        wp_pures.
-        wp_apply (SI_write_spec $! _ _ _ _ (SerVal #2) with "[] [Hx]"). 
-        set_solver.
-        {
-          rewrite !big_sepM_insert; try set_solver.
-          rewrite big_sepM_empty. iDestruct "Hx" as "[[? ?] _]". iFrame.
-        }
-        iIntros "Hcx". wp_pures.
+    wp_apply (simple_wait_transaction_spec _ _ (#1) _ {["x"]} _ (⊤ ∖ ↑client_inv_name)
+      with "[] [] [] [] [] [$Hcstate] [HΦ Htok]"); 
+      [solve_ndisj | iPureIntro; set_solver |  iPureIntro; set_solver | | |].
+    - iModIntro. 
+      iInv (client_inv_name) as ">[%hx' [Hkx Hrest]]" "HClose".
+      iModIntro.
+      iExists {["x":= hx']}.
+      iSplit. 
+      { iPureIntro. set_solver. }
+      iSplitL "Hkx".
+      { rewrite !big_sepM_insert; set_solver. }
+      iIntros "!> Hkx". 
+      iMod ("HClose" with "[Hkx Hrest]") as "_"; try done.
+      iNext. iExists _. 
+      rewrite !(big_sepM_insert); try set_solver.
+      iDestruct "Hkx" as "[Hkx _]". iFrame.
+    - iIntros (v Φ') "!>Htrue HΦ".
+      wp_lam. wp_op.
+      apply bin_op_eval_eq_val.
+      case_bool_decide as Heq;
+      iApply "HΦ"; set_solver.
+    - iIntros (h) "!> (Hcstate & Hseenx)".
+      wp_pures.
+      wp_apply (SI_start_spec $! rpc client_2_addr (⊤ ∖ ↑client_inv_name)); try solve_ndisj.
+      iInv (client_inv_name) as ">[%hx [Hkx [(_ & _ & Htok') | [ (-> & Htok') | -> ]]]]" "HClose".
+      + iDestruct (token_exclusive with "Htok Htok'") as "[]".
+      + iModIntro. iFrame.
+        iExists {["x" := [(#1)]]}.
+        rewrite !big_sepM_insert; try set_solver.
+        rewrite big_sepM_empty.
+        iSplitL "Hkx"; first iFrame.
+        iNext. iIntros "(Hcstate & [Hkx _] & [Hcx _] & _)".
+        iMod ("HClose" with "[Hkx Htok']") as "_".
+        { iNext. iExists [(#1)]. iFrame. set_solver. }
+        iModIntro. wp_pures.
+        wp_apply (SI_write_spec $! _ _ _ _ (SerVal #2) with "[] [Hcx]"). 
+        set_solver. iFrame. iIntros "Hcx". wp_pures.
         wp_apply (commitT_spec rpc client_2_addr (⊤ ∖ ↑client_inv_name));
         try solve_ndisj.
-        iInv (client_inv_name) as ">[%hx' [Hkx [(_ & _ & Htok') | [(-> & Htok') | ->]]]]" "HClose".
-        + iDestruct (token_exclusive with "Htok Htok'") as "[]".
-        + iModIntro. iExists {["x" := [(#1)]]}, _, {["x" := (Some #2, true)]}.
+        iInv (client_inv_name) as ">[%hx [Hkx [(_ & _ & Htok') | [ (-> & Htok') | -> ]]]]" "HClose".
+        * try iDestruct (token_exclusive with "Htok Htok'") as "[]".
+        * iModIntro.
+          iExists {["x" := [(#1)]]}, _, {["x" := (Some (#2), true)]}.
           iFrame. iSplitL "Hcx Hkx". 
-          * iSplitR "Hcx Hkx"; try iSplitR "Hcx Hkx";
-            try iPureIntro; try set_solver.
-            rewrite !big_sepM_insert; try set_solver.
-            rewrite !big_sepM_empty. iFrame.
-          * iNext. iIntros "[_ HBig]". 
-            iMod ("HClose" with "[HBig Htok Htok']") as "_".
-            -- iNext. iExists [(#2);(#1)]. 
-               rewrite !(big_sepM2_insert); try set_solver.
-               iDestruct "HBig" as "[[Hx _] _]".
-               iFrame. iLeft. by iFrame.
-            -- iModIntro. by iApply "HΦ".
-        + rewrite !big_sepM_insert; last set_solver.
-        iDestruct "Hseen" as "[Hseen _]". 
-        iDestruct (Seen_valid (⊤ ∖ ↑client_inv_name) with "[]") as "Hfalse"; 
-        [solve_ndisj|iApply SI_GlobalInv|].
-        iMod ("Hfalse" with "[$Hseen $Hkx]") as "(Kkx & %Hfalse)".
-        destruct Hfalse as [? Hfalse].
-        by apply app_cons_not_nil in Hfalse.
+            -- iSplitR "Hcx Hkx"; try iSplitR "Hcx Hkx";
+              try iPureIntro; try set_solver.
+              rewrite !big_sepM_insert; try set_solver.
+              rewrite !big_sepM_empty. iFrame.
+            -- iNext. iIntros "[_ HBig]". 
+              iMod ("HClose" with "[HBig Htok Htok']") as "_".
+                  ++ iNext. iExists [(#2); (#1)]. 
+                    rewrite !(big_sepM2_insert); try set_solver.
+                    iDestruct "HBig" as "[[Hx _] _]".
+                    iFrame. iLeft. by iFrame.
+                  ++ iModIntro. by iApply "HΦ".
+        * iMod (Seen_valid $! SI_GlobalInv with "[$Hseenx $Hkx]") as "(_ & %Hfalse)";
+          first solve_ndisj.
+          by apply suffix_nil_inv in Hfalse.
+      + iMod (Seen_valid $! SI_GlobalInv with "[$Hseenx $Hkx]") as "(_ & %Hfalse)";
+        first solve_ndisj.
+        by apply suffix_nil_inv in Hfalse.
   Qed.
 
 End proofs.
